cava incr device with separate VALUE/STATUS registers

investigations/bedrock2/IncrementWait/Constants.v
@@ -6,10 +6,11 @@ Local Open Scope string_scope.
 Definition READ := "MMIOREAD".
 Definition WRITE := "MMIOWRITE".
 
-Definition VALUE_ADDR: Z := 16 * 2^10.
-Definition STATUS_ADDR: Z := 16 * 2^10 + 4.
+Definition INCR_BASE_ADDR: Z := 16 * 2^10.
+Definition VALUE_ADDR: Z := INCR_BASE_ADDR.
+Definition STATUS_ADDR: Z := INCR_BASE_ADDR + 4.
+Definition INCR_END_ADDR: Z := INCR_BASE_ADDR + 8.
 
 Definition STATUS_IDLE: Z := 0.
 Definition STATUS_BUSY: Z := 1.
 Definition STATUS_DONE: Z := 2.
-
