investigations/bedrock2/RiscvMachineWithCavaDevice/DetIncrMachine.v
@@ -12,69 +12,138 @@ Section WithCava.
     ctrl <- packV (Vector.of_list [cond]);;
     indexAt branches ctrl.
 
-  (* no input/output, everything is state *)
-  Definition incr_update: unit * (signal (Vec Bit 32)) ->
-                    cava (unit * (signal (Vec Bit 32))) :=
-    fun '(_, state) =>
-      done <- Vec.hd state;;
-      value <- Vec.tl state;;
-      done' <- ret (constant true);;
-      value_r <- Vec.rev value;;
-      value_plus_one_r <- incrN value_r;;
-      value_plus_one <- Vec.rev value_plus_one_r;;
-      value' <- ite done value value_plus_one;;
-      state' <- Vec.cons done' value';;
-      ret (tt, state').
+  (* we need to add the Void because * is left-associative *)
+  Definition void_and_state: Type :=
+    (signal Void * signal Bit * signal Bit * signal Bit * signal Bit * signal Bit *
+     signal (Vec Bit 32) * signal (Vec Bit 32) * signal Bit).
 
-  Definition incr: Circuit unit unit := Loop (Comb incr_update).
+  (* no input/output, everything is state *)
+  Definition incr_update: void_and_state -> cava (void_and_state) :=
+    fun '(dummy_tt, pending_inp, outp_switch, idle, busy, done, value, output, output_en) =>
+      pending_inp' <- constant false;;
+      no_pending_inp <- inv pending_inp;;
+      idle' <- and2 (idle, no_pending_inp);;
+      busy' <- pending_inp;;
+      done' <- or2 (busy, done);;
+      value_plus_one <- incrN value;;
+      value' <- ite busy value_plus_one value;;
+      zeros <- Vec.const (constant false) 29;;
+      v1 <- Vec.cons done zeros;;
+      v2 <- Vec.cons busy v1;;
+      v3 <- Vec.cons idle v2;;
+      output_en' <- constant true;;
+      output' <- ite outp_switch value v3;;
+      ret (dummy_tt, pending_inp', outp_switch, idle', busy', done', value', output', output_en').
+
+  Definition incr: Circuit (signal Void) (signal Void) :=
+    Loop (Loop (Loop (Loop (Loop (Loop (Loop (Loop (Comb incr_update)))))))).
 
 End WithCava.
 
-Definition device_state := Vector.t bool 32.
+Definition device_state: Type := Eval simpl in circuit_state incr.
 
-(*
-Eval simpl in circuit_state incr.
-*)
+Definition get_output: device_state -> Vector.t bool 32 :=
+  fun '(_, (_, (_, (_, (_, (_, (_, (_, (_, output_en), output),
+                                value), done), busy), idle), outp_switch), pending_inp)) => output.
+
+Definition get_output_en: device_state -> bool :=
+  fun '(_, (_, (_, (_, (_, (_, (_, (_, (_, output_en), output),
+                                value), done), busy), idle), outp_switch), pending_inp)) => output_en.
+
+Definition get_pending_inp: device_state -> bool :=
+  fun '(_, (_, (_, (_, (_, (_, (_, (_, (_, output_en), output),
+                                value), done), busy), idle), outp_switch), pending_inp)) => pending_inp.
+
+Definition set_outp_switch(b: bool): device_state -> device_state :=
+  fun '(_, (_, (_, (_, (_, (_, (_, (_, (_, output_en), output),
+                                value), done), busy), idle), outp_switch), pending_inp)) =>
+    (tt, (tt, (tt, (tt, (tt, (tt, (tt, (tt, (tt, output_en), output),
+                                   value), done), busy), idle), b), pending_inp)).
+
+Definition set_outp_en(b: bool): device_state -> device_state :=
+  fun '(_, (_, (_, (_, (_, (_, (_, (_, (_, output_en), output),
+                                value), done), busy), idle), outp_switch), pending_inp)) =>
+    (tt, (tt, (tt, (tt, (tt, (tt, (tt, (tt, (tt, b), output),
+                                   value), done), busy), idle), outp_switch), pending_inp)).
+
+Definition set_pending_inp(b: bool): device_state -> device_state :=
+  fun '(_, (_, (_, (_, (_, (_, (_, (_, (_, output_en), output),
+                                value), done), busy), idle), outp_switch), pending_inp)) =>
+    (tt, (tt, (tt, (tt, (tt, (tt, (tt, (tt, (tt, output_en), output),
+                                   value), done), busy), idle), outp_switch), b)).
+
+Definition set_value(v: Vector.t bool 32): device_state -> device_state :=
+  fun '(_, (_, (_, (_, (_, (_, (_, (_, (_, output_en), output),
+                                value), done), busy), idle), outp_switch), pending_inp)) =>
+    (tt, (tt, (tt, (tt, (tt, (tt, (tt, (tt, (tt, output_en), output),
+                                   v), done), busy), idle), outp_switch), pending_inp)).
 
 Definition incr_device_step(state: device_state): device_state :=
-  snd (snd (fst (step incr (tt, (tt, state)) tt))).
+  fst (step incr state tt).
 
-(*
-Compute incr_device_step (Vector.const false 1 ++ Vector.const false 28 ++ Vector.const true 3)%vector.
-*)
+Require Import coqutil.Datatypes.List.
+
+Example sample_trace := Eval compute in
+  let done := false in
+  let busy := false in
+  let idle := true in
+  let outp_switch := false in
+  let pending_inp := true in
+  let output := Vector.const false 32 in
+  let output_en := false in
+  let value := (Vector.const true 2 ++ Vector.const false 30)%vector in
+  let start := (tt, (tt, (tt, (tt, (tt, (tt, (tt, (tt, (tt,
+      output_en), output), value), done), busy), idle), outp_switch), pending_inp)) in
+  List.unfoldn incr_device_step 5 start.
+
+(* Print sample_trace. *)
 
 Require Import Coq.ZArith.ZArith. Open Scope Z_scope.
 Require Import riscv.Utility.Utility.
 Require Import coqutil.Map.Interface.
 Require Import coqutil.Map.Properties.
 Require Import Bedrock2Experiments.RiscvMachineWithCavaDevice.InternalMMIOMachine.
+Require Import Bedrock2Experiments.IncrementWait.Constants.
 
 Section WithParameters.
   Context {word: Interface.word 32} {word_ok: word.ok word}
           {Mem: map.map word byte} {Registers: map.map Z word}.
 
-  Definition INCR_DEVICE_ADDR: word := word.of_Z (16 * 2^10).
-
-  (* we want the msb to be the head, and we use Cava's reverse rather than Coq's reverse
-     because Coq's contains opaque proof terms *)
-
   Definition bv_to_word(v: Vector.t bool 32): word :=
-    word.of_Z (Z.of_N (Bv2N (Cava.Util.Vector.reverse v))).
+    word.of_Z (Z.of_N (Bv2N v)).
 
   Definition word_to_bv(w: word): Vector.t bool 32 :=
-    Cava.Util.Vector.reverse (N2Bv_sized 32 (Z.to_N (word.unsigned w))).
+    N2Bv_sized 32 (Z.to_N (word.unsigned w)).
 
   Global Instance counter_device: device := {|
     device.state := device_state;
-    device.reset_state := word_to_bv (word.of_Z 0);
+
+    device.reset_state :=
+      (tt, (tt, (tt, (tt, (tt, (tt, (tt, (tt, (tt, false),
+                                          word_to_bv (word.of_Z 0)), word_to_bv (word.of_Z 0)),
+                                false), false), true), false), false));
+
     device.run1 := incr_device_step;
-    device.addr_range_start := INCR_DEVICE_ADDR;
-    device.addr_range_pastend := word.add INCR_DEVICE_ADDR (word.of_Z 4);
-    device.readReq(num_bytes: nat)(addr: word)(s: device_state) := s;
-    device.readResp(s: device_state) := Some (bv_to_word s);
-    device.writeReq(num_bytes: nat)(addr value: word)(s: device_state) := word_to_bv value;
-    device.writeResp(s: device_state) := Some tt;
-    device.maxRespDelay := 0;
+
+    device.addr_range_start := word.of_Z INCR_BASE_ADDR;
+    device.addr_range_pastend := word.of_Z INCR_END_ADDR;
+
+    device.readReq(num_bytes: nat)(addr: word)(s: device_state) :=
+      (* TODO the address-to-register mapping could/should also be implemented in Cava *)
+      set_outp_en false (set_outp_switch (word.eqb (word.of_Z 0) (word.and addr (word.of_Z 4))) s);
+      (* outp_en will be set to true as soon as one cycle is run, which can set output
+         according to outp_switch *)
+
+    device.readResp(s: device_state) :=
+      if get_output_en s then Some (bv_to_word (get_output s)) else None;
+
+    device.writeReq(num_bytes: nat)(addr value: word)(s: device_state) :=
+      set_value (word_to_bv value) (set_pending_inp true s);
+
+    device.writeResp(s: device_state) :=
+      if get_pending_inp s then None else Some tt;
+
+    device.maxRespDelay := 1;
   |}.
 
 End WithParameters.
